\documentclass[11pt,letterpaper]{article}
\usepackage{amsmath}
\usepackage{amssymb}
\usepackage{fullpage}
\usepackage{enumerate}

\title{CS 70, Summer 2014 --- Homework 2} % Put the correct homework number here.
\author{Harsimran (Sammy) Sidhu, SID 23796591} % Put your name and student ID here.

\begin{document}

\maketitle

Collaboraters: Chonyi Lama, Jenny Pushkarskaya

Sources: http://comet.lehman.cuny.edu/sormani/teaching/induction.html

\section*{Problem 1} % Put the correct problem number here

\begin{enumerate}[(a)]
%8a
\item
$\forall n>0$\\
 $\left[ {\begin{array}{cc}
   1 & 2 \\
   0 & 1 \\
  \end{array} } \right]^n 
  \leq 
   \left[ {\begin{array}{cc}
   2n & 2n \\
   2n & 2n \\
  \end{array} } \right]$\\
  \\
  Proof: Define $A(x)$ to be\\\\
   $\left[ {\begin{array}{cc}
   1 & 2 \\
   0 & 1 \\
  \end{array} } \right]^n$ \\
  
  Base Cases:\\
  let $n=1$\\\\
  $A(1) = 
   \left[ {\begin{array}{cc}
   1 & 2 \\
   0 & 1 \\
  \end{array} } \right]$\\\\
   $\left[ {\begin{array}{cc}
   1 & 2 \\
   0 & 1 \\
  \end{array} } \right]
  \leq    \left[ {\begin{array}{cc}
   2 & 2 \\
   2 & 2 \\
  \end{array} } \right]$\hfill Valid\\
  
  
  
  let $n=2$\\\\
  $A(2) = 
   \left[ {\begin{array}{cc}
   1 & 2 \\
   0 & 1 \\
  \end{array} } \right]^2
  =
  \left[ {\begin{array}{cc}
   1 & 2 \\
   0 & 1 \\
  \end{array} } \right]
  \times
  \left[ {\begin{array}{cc}
   1 & 2 \\
   0 & 1 \\
  \end{array} } \right]
  =
  A(1)\times
   \left[ {\begin{array}{cc}
   1 & 2 \\
   0 & 1 \\
  \end{array} } \right]
  =
   \left[ {\begin{array}{cc}
   1 & 4 \\
   0 & 1 \\
  \end{array} } \right]$\\\\
  
   $\left[ {\begin{array}{cc}
   1 & 4 \\
   0 & 1 \\
  \end{array} } \right]
  \leq    \left[ {\begin{array}{cc}
   4 & 4 \\
   4 & 4 \\
  \end{array} } \right]$\hfill Valid\\
  
  let $n =3$\\\\
  $A(3) = 
  \left[ {\begin{array}{cc}
   1 & 2 \\
   0 & 1 \\
  \end{array} } \right]^3
  =
  A(2)\times
   \left[ {\begin{array}{cc}
   1 & 2 \\
   0 & 1 \\
  \end{array} } \right]
  =
   \left[ {\begin{array}{cc}
   1 & 6 \\
   0 & 1 \\
  \end{array} } \right]\\\\
   \left[ {\begin{array}{cc}
   1 & 6 \\
   0 & 1 \\
  \end{array} } \right]
  \leq    \left[ {\begin{array}{cc}
   6 & 6 \\
   6 & 6 \\
  \end{array} } \right]$\hfill Valid\\\\
  Strengthing the Hypothesis: From the base cases it seems that\\\\
  $A(n) = 
  \left[ {\begin{array}{cc}
   1 & 2 \\
   0 & 1 \\
  \end{array} } \right]^n 
  = 
  \left[ {\begin{array}{cc}
   1 & 2n \\
   0 & 1 \\
  \end{array} } \right]\\\\
   $
Which is obviously $(\leq2n)$ for every entry.\\\\
Inductive~Hypothesis:
$A(k) = 
  \left[ {\begin{array}{cc}
   1 & 2 \\
   0 & 1 \\
  \end{array} } \right]^k 
  = 
  \left[ {\begin{array}{cc}
   1 & 2k \\
   0 & 1 \\
  \end{array} } \right]\\
   $\\
   let $n=k+1\\\\
\left[ {\begin{array}{cc}
   1 & 2 \\
   0 & 1 \\
  \end{array} } \right]^{k+1} 
  = 
  \left[ {\begin{array}{cc}
   1 & 2(k+1) \\
   0 & 1 \\
  \end{array} } \right]$\\
  
  
  
 
   $\left[ {\begin{array}{cc}
   1 & 2 \\
   0 & 1 \\
  \end{array} } \right]^{k}
  \times 
   \left[ {\begin{array}{cc}
   1 & 2 \\
   0 & 1 \\
  \end{array} } \right]
  = 
  \left[ {\begin{array}{cc}
   1 & 2k+2 \\
   0 & 1 \\
  \end{array} } \right]\\
   $
   

   $\left[ {\begin{array}{cc}
   1 & 2k \\
   0 & 1 \\
  \end{array} } \right]
  \times 
   \left[ {\begin{array}{cc}
   1 & 2 \\
   0 & 1 \\
  \end{array} } \right]
  = 
  \left[ {\begin{array}{cc}
   1 & 2k+2 \\
   0 & 1 \\
  \end{array} } \right]$\hfill Substitute Inductive Hypothesis\\



 $\left[ {\begin{array}{cc}
   (1\times 1 + 0\times 2k) & (1\times2 + 2k\times1) \\
   (0\times1 + 1\times0) & (0\times2 + 1\times 1) \\
  \end{array} } \right]
  = 
  \left[ {\begin{array}{cc}
   1 & 2k+2 \\
   0 & 1 \\
  \end{array} } \right]$\\

 $\left[ {\begin{array}{cc}
   1 & 2k + 2 \\
   0 & 1 \\
  \end{array} } \right]
  = 
  \left[ {\begin{array}{cc}
   1 & 2k+2 \\
   0 & 1 \\
  \end{array} } \right]$\hfill Valid\\

%8b
\item

$\forall c\geq 12~\exists(m,n)\in\mathbb{N}~(3m + 7n = c)$\hfill Original Statement\\
$m$ is the number of 3 cent coins and $n$ is the number of 7 cent coins\\
Base Cases:\\
$(c=12)\rightarrow (m=4,n=0)\rightarrow (3(4) + 7(0) = 12)$\\
$(c=13)\rightarrow (m=2,n=1)\rightarrow (3(2) + 7(1) = 13)$\hfill (m=m-2,~n=n+1)\\
$(c=14)\rightarrow (m=0,n=2)\rightarrow (3(0) + 7(2) = 14)$\hfill (m=m-2,~n=n+1)\\\\
Inductive Hypothesis: Suppose we can make form any integer value of cents from $12$ to $k$. We need to show that we can make $k+1$ cents using only 3-cent and 7-cent coins\\\\
Since we proved base cases to 14, we'll assume $k+1\geq 15$\\
$k+1\geq 15$\\
$(k+1)-3\geq 15-3$\\
$(k+1)-3\geq 15-3$\\
$(k+1)-3\geq 12$\\
$(k+1)-3=3m +7n$\\
$(k+1)=3(m+1) +7n$\hfill valid\\
\clearpage
%8c
\item
$\forall n\in\mathbb{N}~(F_n = \frac{\phi^n-(1-\phi)^n}{\sqrt{5}})$ where $\phi = \frac{1+\sqrt{5}}{2}$\\
$(F_n = F_{n-2} +F_{n-1})$ where $F_0 = 0,~F_1 =1$\\
\\
Proof: $F_n = \frac{\phi^n-(1-\phi)^n}{\sqrt{5}}= F_{n-2} +F_{n-1}$\\
\\
Base~Cases:\\
$n=0\rightarrow \frac{\phi^0-(1-\phi)^0}{\sqrt{5}} = 0$\hfill True\\
$n=1\rightarrow \frac{\phi^1-(1-\phi)^1}{\sqrt{5}} = \frac{\phi- 1+\phi}{\sqrt{5}}=\frac{2\phi -1}{\sqrt{5}}=\frac{1+\sqrt{5}-1}{\sqrt{5}}=1$\hfill True\\
Inductive~Hypothesis: Assume $F_k = \frac{\phi^k-(1-\phi)^k}{\sqrt{5}}$ is true for integers $0 \leq k$\\
We now need to show $F(k)$ for $k\geq2$\\
$let~n=k+2$ \hfill Will hit either of the two base cases\\
\\
$F_{k+2} = \frac{\phi^{k+2}-(1-\phi)^{k+2}}{\sqrt{5}}
= \frac{\phi^2\phi^{k}-(1-\phi)^{2}(1-\phi)^{k}}{\sqrt{5}}$\hfill Factor out\\
$\phi^2 = (\frac{1+\sqrt{5}}{2})^2=\frac{6}{4}+\frac{\sqrt{5}}{2}=1 +\frac{1+\sqrt{5}}{2}
= 1+\phi$\\
$(1-\phi)^2=(1-\frac{1+\sqrt{5}}{2})^2=(\frac{1-\sqrt{5}}{2})^2=\frac{6}{4}-\frac{\sqrt{5}}{2}=1+\frac{1-\sqrt{5}}{2}=(1+(1-\phi))$\\
\\
$F_{k+2} = \frac{\phi^{k}(1+\phi)-(1-\phi)^{k}(1+(1-\phi))}{\sqrt{5}}
= \frac{\phi^{k}+\phi^{k+1}-(1-\phi)^{k}-(1-\phi)^{k+1}}{\sqrt{5}}$\hfill Simplify\\
$F_{k+2} =\frac{\phi^{k}-(1-\phi)^{k}}{\sqrt{5}} + 
\frac{\phi^{k+1}-(1-\phi)^{k+1}}{\sqrt{5}}\hfill$ Group by order\\
$F_{k+2} = F_{k} +F_{k+1}$\hfill Substitute hypothesis\\
$F_k = F_{k-2}+F_{k-1}\hfill$ Valid

%8d
\item
$\forall n\geq2\in\mathbb{N}~f(n)=7f(n-1)-10f(n-2)$ where $f(0) = 1,~ f(1) = 2$\\
$table~f(n)$\\
$f(0) = 1$\hfill True\\
$f(1) =2$\hfill True\\
$f(2)=4$\\
$f(3)=8$\\
$f(4)=16$\\\\
Proof:
$f(n)=7f(n-1)-10f(n-2)=2^n$ with Induction on $n$\hfill Fits the table\\
Inductive~hypothesis: Assume $f(k)=2^k$ for all $n$ between 2 and $k$. We now need to show that $f(k+1) = 2^{k+1}$\\
\\
$let~n=k+1$\\
$f(k+1)=7f(k)-10f(k-1)=7\times2^{k}-10\times2^{k-1}$\hfill Substitute hypothesis\\
$f(k+1)=7f(k)-10f(k-1)=7\times2^{k}-10\times2^{k-1}$\\
$f(k+1)=7f(k)-10f(k-1)=7\times2^{k}-5\times2^{k}$\\
$f(k+1)=7f(k)-10f(k-1)=2\times2^{k}$\\
$f(k+1)=7f(k)-10f(k-1)=2^{k+1}$\\
$f(k+1) = 2^{k+1}$\hfill Valid\\

\end{enumerate}
\clearpage

\section*{Problem 2}
\begin{enumerate}[(a)]
\item
True, if man $M$ and woman $W$ put each other on top of their respective preference list and they are both paired with other people then they will always be a rogue couple.\\
\item
False, if man $M$ and woman $W$ are on the bottom of everyone's preference list then they would be paired to one another with no rogue couples existing.\\
\item
True, there exists a stable marriage instance where every unmatched couple is a rogue couple. If all the men were matched to their unique least preferred woman and the the women also preferred that man the least uniquely then every couple would be a rogue couple.\\
\end{enumerate} 
\clearpage

\section*{Problem 3}
\begin{enumerate}[(a)]
\item
\textbf{Every Morning:} Each student goes to the hospital on top of their list that they haven't  crossed off yet\\
\\
\textbf{Every Afternoon:} Each hospital $h$ says to come back the next day to the top $q_h$ students (from prior day's waitlist and new proposals) and adds them to their waitlist. Then each hospital $h$ rejects their respective non-top students that were proposals or prior waitlisters that are no longer in the top $q_h$ and have been bumped out.\\
\\
\textbf{Every Night:} Each rejected student then crosses off the hospital $h$ that rejected them.\\
\\
The loop is repeated until no more students are rejected from hospitals and all the slots for have been filled for each hospital $h$. Each hospital $h$ now accepts the $q_h$ students on their waitlist.\\

\item
\textbf{Improvement Lemma:} For each hospital $h$, after its waitlist becomes full, its least favorite student on the waitlist can only improve over time.
\\
\\
Suppose a proof by contradiction, that hospital $h$'s least favorite student becomes worse with each day. On day $k$ hospital $h$ has a student $s$ that is its least favorite. On day $k+1$, student $s\prime$ proposes to hospital $h$. Since our algorithm states that hospital $h$ bumps off it's least favorite student, student $s$ is rejected. That means that the hospital favors $s\prime$ over $s$ meaning $s\prime > s$. This contradicts our assumption and proves that hospital $h$'s waitlist only improves with time.
\\\\
\textbf{Lemma:} The algorithm must find a stable arrangement.\\
\\
Let's suppose that our algorithm doesn't find a stable arrangement, and there's a rouge student hospital pair $(s,h^*)$. (where $s$ prefers $h^*$ and vice-versa). Let's also say that $s$ is now paired with $h$. For $s$ to get paired with $h$, $s$ must have had to propose to $h^*$, and since $h^*$ prefers $s$, it would have not rejected $s$ from it's waitlist. We have a contradiction here, proving that the algorithm does in fact find a stable arrangement.\\

\end{enumerate}
\clearpage


\section*{Problem 4}
$d=gcd(x,y)=ax+by$\\
\begin{enumerate}[(a)]
\item
$d=gcd(x,y)=(a_0 +yk)x+(b_0-xk)y$\\
$d=gcd(x,y)=a_0 x +xyk+b_0 y-xyk$\\
$d=gcd(x,y)=a_0 x+b_0 y$\\
\\
$\forall k~a=a_0 +yk,~b=b_0-xk$\\
\item
$gcd(30,18)\rightarrow 30 = (1\times18)+12$\\
$gcd(18,12)\rightarrow 18 = (1\times12)+6$\\
$gcd(12,6)\rightarrow 12 = (2\times6)+0$\\
$gcd(6,0)\rightarrow 6 = (0\times0)+6\rightarrow~m=6$\\
\\
extended gcd\\
$d=gcd(x,y)=~~~~~~a_0x+b_0y$\\
$6=gcd(6,0)=~~~~~1(6)+0(0)$\\
$6=gcd(12,6)=~~~0(12)+1(6)$\\
$6=gcd(18,12)=~~1(18)-1(6)$\\
$6=gcd(30,18)=-1(30)+2(18)\rightarrow a_0=-1,~b_0=2$\\
\\
$\forall k~a=-1+18k,~b=2-30k$\\
\item
$d=gcd(x,y)=ax+by$\\
$2d=2ax+2by$\\
$2d=(2a)x+(2b)y$\\
$6=gcd(30,18)=-1(30)+2(18)$\\
$2\times6=(2\times-1)(30)+(2\times2)(18)$\\
$12=-2(30)+4(18)$\\
$(a=-2,~b=4)$
\end{enumerate}
\clearpage
\section*{Problem 5}
\begin{enumerate}[(a)]
%5a
\item
$(3002+6002\times9002)$ mod 3\\
$(2+2\times2)$ mod 3\\
$(2+4)$ mod 3\\
$(6)$ mod 3\\
\\
$0$ mod 3\\
%5b
\item
$(1002^3-2468\times17+4)$ mod 5\\
$(2^3-3\times2+4)$ mod 5\\
$(8-6+4)$ mod 5\\
$(3-1+4)$ mod 5\\
$(6)$ mod 5\\
\\
$(1)$ mod 5\\
%5c
\item
Inverses for $\{0,1,2,... ,19\}$ mod 20\\
gcd$(20,1)=$\
gcd$(20,3)=$\
gcd$(20,7)=$\
gcd$(20,9)=$\
gcd$(20,11)=$\
gcd$(20,13)=$\
gcd$(20,17)=$\
gcd$(20,19)=1$\\
\\
$\{1,3,7,9,11,13,17,19\}$ have inverses mod 20\\
\\
$1 = 1b$ mod 20 $let~ b =21$\\
$1=3b$ mod 20 $let~ b =7$\\
$1=7b$ mod 20 $let~ b =3$\\
$1=9b$ mod 20 $let~ b =9$\\
$1=11b$ mod 20 $let~ b =-9$\\
$1=13b$ mod 20 $let~ b =-3$\\
$1=17b$ mod 20 $let~ b =-7$\\
$1=19b$ mod 20 $let~ b =-1$\\
\clearpage
%5d
\item
$\dfrac{5-(19\times3)}{7\times9}$ mod 20\\
\\
$=\dfrac{5-57}{63}$ mod 20\\
\\
$=\dfrac{5+3}{3}$ mod 20\\
\\
$=\dfrac{8}{3}$ mod 20\\
\\
$= 8\times3^{-1}$ mod 20\\
$= 8\times7$ mod 20\hfill inverse found in 5c\\
$= 56$ mod 20\\
$= 16$ mod 20\\
%5e
\item
$1=$gcd$(m,x)=am+bx$\\
gcd$(55,36)$\\
gcd$(55,36)\rightarrow55 = 1(36) + 19$\\
gcd$(36,19)\rightarrow36 = 1(19)+ 17$\\
gcd$(19,17)\rightarrow19 = 1(17)+ 2$\\
gcd$(17,2)\rightarrow17 = 8(2)+ 1$\\
gcd$(2,1)\rightarrow2 = 2(1)+ 0$\\
gcd$(1,0)\rightarrow1 = 0(0)+ 1$\\
\\
Extended gcd for the inverse\\
$1=$gcd$(m,x)=am+bx$\\
gcd$(1,0)=1= 1(1)+ 0(0)$\\
gcd$(2,1)=1 = 0(2)+ 1(1)$\\
gcd$(17,2)=1 = 1(17)- 8(2)$\\
gcd$(19,17)=1 = -8(19) + 9(17)$\\
gcd$(36,19)=1 = 9(36) + -17(19)$\\
gcd$(55,36)=1 = -17(55) + 26(36)$  $b=26$\\
$36^{-1}$ mod 55 = \textbf{26}\\
$(26\times36)$ mod 55 $=(936)$ mod 55 $=(1)$ mod 55\hfill valid\\
%5f
\item
$17x\equiv4$ mod 20\\
$(-7)\times17x\equiv(-7)\times4$ mod 20\hfill inverse found in 5c\\
$-119x\equiv-28$ mod 20\\
\\
$x\equiv12$ mod 20\\
$\forall k\in\mathbb{Z}~x=12+20k$\\
\clearpage
%5g
\item
$5x+3y\equiv0$ (mod 19)\\
$y\equiv4+12x$ (mod 19)\\
$5x+3y\equiv0$ (mod 19) $\rightarrow$ $3y\equiv-5x$ (mod 19)\\ 
$\rightarrow$ $(-6)\times3y\equiv(-6)\times-5x$ (mod 19)\\
$\rightarrow$ $-18y\equiv30x$ (mod 19)\\
$\rightarrow$ $y\equiv11x$ (mod 19)\\
$11x\equiv4+12x$ (mod 19)\\
$0\equiv4+x$ (mod 19)\\
$-4\equiv x$ (mod 19)\\
$x\equiv 15$ (mod 19)\\
$y\equiv11(15)$ (mod 19)\\
$y\equiv165$ (mod 19)\\
$y\equiv13$ (mod 19)\\
\\
$x\equiv 15$ (mod 19)\\
$y\equiv13$ (mod 19)\\

\end{enumerate}
\clearpage

\section*{Problem 6}
\begin{enumerate}[(a)]
\item

\end{enumerate}


\end{document}

